Add requirement patterns and proofs

Pattern7_Def.thy
@@ -1,5 +1,5 @@
 theory Pattern7_Def
-  imports VCTheoryLemmas
+  imports Pattern2_Def
 begin
 
 definition P7inv where "P7inv s T T1 a1 a2 a3\<equiv>
@@ -57,5 +57,198 @@ lemma einv2req: "P7inv s t t1 A1 A2 A3 \<Longrightarrow> P7 s t A1 A2 A3"
   apply auto
   done
 
+definition constrained_weak_until where "constrained_weak_until s1 s t A1 A2 \<equiv>
+(\<exists> s4. toEnvP s4 \<and> substate s1 s4 \<and> substate s4 s \<and> toEnvNum s1 s4 \<le> t \<and> A2 s4 \<and>
+(\<forall> s3. toEnvP s3 \<and> substate s1 s3 \<and> substate s3 s4 \<and> s3 \<noteq> s4 \<longrightarrow> A1 s3)) \<or>
+(\<forall> s3. toEnvP s3 \<and> substate s1 s3 \<and> substate s3 s \<and> toEnvNum s1 s3 \<le> t \<longrightarrow> A1 s3)"
+
+definition constrained_weak_until_inv where "constrained_weak_until_inv s1 s t t1 A1 A2 \<equiv>
+(\<exists> s4. toEnvP s4 \<and> substate s1 s4 \<and> substate s4 s \<and> toEnvNum s1 s4 \<le> t \<and> A2 s4 \<and>
+(\<forall> s3. toEnvP s3 \<and> substate s1 s3 \<and> substate s3 s4 \<and> s3 \<noteq> s4 \<longrightarrow> A1 s3)) \<or>
+toEnvNum s1 s \<ge> t1 \<and>
+(\<forall> s3. toEnvP s3 \<and> substate s1 s3 \<and> substate s3 s \<and> toEnvNum s1 s3 \<le> t \<longrightarrow> A1 s3)"
+
+lemma constrained_weak_until_one_point: "toEnvP s \<Longrightarrow> A2 s \<or> t1 = 0 \<and> A1 s \<Longrightarrow> constrained_weak_until_inv s s t t1 A1 A2"
+  apply(unfold constrained_weak_until_inv_def)
+  by (metis substate_antisym substate_refl toEnvNum_id zero_le)
+
+lemma constrained_weak_until_rule: " consecutive s0 s \<Longrightarrow>
+(\<forall> s1. toEnvP s1 \<and> substate s1 s0 \<and> A1 s1 \<longrightarrow> A1' s1) \<and>
+(\<forall> s1. toEnvP s1 \<and> substate s1 s0 \<and> A2 s1 \<longrightarrow> A2' s1) \<and>
+(t1 < t \<and> (A2' s \<and>  t1' \<le> t+1  \<or>  t1' \<le> t1 + 1 \<and> A1' s) \<or> t1 \<ge> t \<and> t1' \<le> t1 + 1) \<Longrightarrow>
+(\<forall> s1. toEnvP s1 \<and> substate s1 s0 \<and> constrained_weak_until_inv s1 s0 t t1 A1 A2 \<longrightarrow> constrained_weak_until_inv s1 s t t1' A1' A2')"
+  apply(unfold constrained_weak_until_inv_def)
+  apply(rule allI)
+  subgoal for s1
+    apply(rule impI)
+    apply(erule conjE)+
+    apply(rotate_tac -1)
+    apply(erule disjE)
+     apply (metis consecutive.simps substate_trans)
+    apply(erule disjE)
+     apply(erule conjE)+
+     apply(erule disjE)
+    apply(cases "toEnvNum s1 s0 < t")
+      apply(rule disjI1)
+      apply(rule exI[of _ s])
+      apply(rule conjI)
+       apply simp
+      apply(rule conjI)
+       apply (meson consecutive.elims(2) substate_trans)
+      apply(rule conjI)
+       apply simp
+      apply(rule conjI)
+        apply (metis Suc_eq_plus1 add_mono1 consecutive.simps less_Suc_eq_le toEnvNum3)
+       apply(rule conjI)
+        apply simp
+       apply (metis consecutive.elims(2) le_Suc_ex less_or_eq_imp_le substate_noteq_imp_substate_of_pred toEnvNum3 trans_le_add1)
+    apply(rule disjI2)
+      apply (smt (verit, ccfv_SIG) add.commute consecutive.elims(2) leD leI le_iff_add le_neq_implies_less le_numeral_extra(4) le_trans less_add_one nat_add_left_cancel_le nat_le_linear order.strict_trans1 substate_noteq_imp_substate_of_pred toEnvNum3)
+    apply (smt (verit, best) add.commute consecutive.elims(2) nat_add_left_cancel_le order_subst1 substate_noteq_imp_substate_of_pred toEnvNum3)
+    apply(rule disjI2)
+    apply(rule conjI)
+    using toEnvNum3 apply fastforce
+    by (metis consecutive.elims(2) dual_order.trans leD less_add_one substate_noteq_imp_substate_of_pred toEnvNum3)
+  done
+
+lemma constrained_weak_until_einv2req: "
+(\<forall> s1. toEnvP s1 \<and> substate s1 s \<and> A1 s1 \<longrightarrow> A1' s1) \<and>
+(\<forall> s1. toEnvP s1 \<and> substate s1 s \<and> A2 s1 \<longrightarrow> A2' s1) \<Longrightarrow>
+(\<forall> s1. toEnvP s1 \<and> substate s1 s \<and> constrained_weak_until_inv s1 s t t1 A1 A2 \<longrightarrow> constrained_weak_until s1 s t A1' A2')"
+  apply(unfold constrained_weak_until_inv_def constrained_weak_until_def)
+  by (meson substate_trans)
+
+definition P7_2 where "P7_2 s t A1 A2 A3 A4 A5 \<equiv>
+always2 s A1 A2 (\<lambda> s2. constrained_weak_until s2 s t A3 (\<lambda> s4. previous_ex s4 A4 \<and> A5 s4))"
+
+definition P7_2inv where "P7_2inv s t t1 b1 b2 A1 A2 A3 A4 A5 \<equiv>
+always2 s A1 A2 (\<lambda> s2. constrained_weak_until_inv s2 s t t1 A3 (\<lambda> s4. previous_ex s4 A4 \<and> A5 s4)) \<and> (b1 = A1 s) \<and> (b2 = A4 s)" 
+
+lemma P7_2_rule: "consecutive s0 s \<Longrightarrow>
+P7_2inv s0 t t1 b1 b2 A1 A2 A3 A4 A5 \<and> (\<not> b1 \<or> \<not> A2 s  \<or> b2 \<and> A5 s \<or> t1' = 0 \<and> A3 s) \<and> 
+(t1 < t \<and> (b2 \<and> A5 s \<and>  t1' \<le> t+1  \<or>  t1' \<le> t1 + 1 \<and> A3 s) \<or> t1 \<ge> t \<and> t1' \<le> t1 + 1) \<and> (b1' = A1 s) \<and> (b2' = A4 s) \<Longrightarrow>
+P7_2inv s t t1' b1' b2' A1 A2 A3 A4 A5"
+  apply(unfold P7_2inv_def)
+  apply(rule conjI)
+  subgoal
+    apply(rule always2_rule[of s0])
+     apply simp
+    apply(rule conj_forward)
+      prefer 2
+      apply(rotate_tac -1)
+      apply assumption
+     prefer 2
+     apply(rule conj_forward)
+       prefer 2
+       apply(rule disj_forward)
+         prefer 2
+      apply(rotate_tac -1)
+         apply assumption
+        prefer 2
+        apply(rule disj_forward)
+          prefer 2
+          apply(rotate_tac -1)
+          apply assumption
+         prefer 2
+         apply(rule constrained_weak_until_one_point)
+          apply simp
+         apply(rule disj_forward)
+           prefer 2
+           apply(rule conj_forward)
+             prefer 2
+             apply(rule previous_ex_one_point[of s0])
+              apply simp
+          apply(rotate_tac -1)
+             apply assumption
+            prefer 2
+          apply(rotate_tac -1)
+            apply assumption
+          apply(rotate_tac -1)
+           apply assumption
+          prefer 2
+          apply(rotate_tac -1)
+          apply assumption
+          apply(rotate_tac -1)
+         apply assumption
+          apply(rotate_tac -1)
+        apply assumption
+          apply(rotate_tac -1)
+       apply assumption
+      prefer 2
+      apply(rule constrained_weak_until_rule[of s0])
+       apply simp
+      apply(rule conj_forward)
+        prefer 2
+        apply(rule all_imp_refl)
+          apply(rotate_tac -1)
+        apply assumption
+       prefer 2
+      apply(rule conj_forward)
+        prefer 2
+        apply(rule all_imp_refl)
+          apply(rotate_tac -1)
+        apply assumption
+        prefer 2
+        apply(rule disj_forward)
+          prefer 2
+          apply(rule conj_forward)
+            prefer 2
+          apply(rotate_tac -1)
+            apply assumption
+           prefer 2
+           apply(rule disj_forward)
+             prefer 2
+             apply(rule conj_forward)
+               prefer 2
+               apply(rule conj_forward)
+                 prefer 2
+                 apply(rule previous_ex_one_point[of s0])
+                  apply simp
+                 apply(rotate_tac -1)
+                 apply assumption
+                apply(rotate_tac -1)
+                apply assumption
+               apply(rotate_tac -1)
+               apply assumption
+              prefer 2
+              apply(rotate_tac -1)
+              apply assumption
+             apply(rotate_tac -1)
+             apply assumption
+            prefer 2
+            apply(rotate_tac -1)
+            apply assumption
+           apply(rotate_tac -1)
+           apply assumption
+          apply(rotate_tac -1)
+          apply assumption
+         prefer 2
+         apply(rotate_tac -1)
+         apply assumption
+        apply(rotate_tac -1)
+        apply assumption
+          apply(rotate_tac -1)
+       apply assumption
+      apply(rotate_tac -1)
+      apply assumption
+     apply(rotate_tac -1)
+     apply assumption
+    apply(erule conjE)+
+    apply auto
+    done
+  apply auto
+  done
+
+lemma P7_2_rule': "
+P7_2inv s0 t t1 b1 b2 A1 A2 A3 A4 A5 \<Longrightarrow> consecutive s0 s \<Longrightarrow> (\<not> b1 \<or> \<not> A2 s  \<or> b2 \<and> A5 s \<or> t1' = 0 \<and> A3 s) \<and> 
+(t1 < t \<and> (b2 \<and> A5 s \<and>  t1' \<le> t+1  \<or>  t1' \<le> t1 + 1 \<and> A3 s) \<or> t1 \<ge> t \<and> t1' \<le> t1 + 1) \<and> (b1' = A1 s) \<and> (b2' = A4 s) \<Longrightarrow>
+P7_2inv s t t1' b1' b2' A1 A2 A3 A4 A5"
+  using P7_2_rule by blast
+
+
+lemma P7_2_einv2req: "P7_2inv s t t1 b1 b2  A1 A2 A3 A4 A5 \<Longrightarrow> P7_2 s t A1 A2 A3 A4 A5"
+  apply(unfold P7_2inv_def P7_2_def)
+  using always2_einv2req constrained_weak_until_einv2req
+  by (smt (verit, ccfv_SIG))
 
 end
