Barrier/Proofs_R1.thy
@@ -1,0 +1,156 @@
+theory Proofs_R1
+  imports CommonExtraInv Requirements  "../VCTheoryLemmas"
+begin
+
+definition inv1 where "inv1 s \<equiv>  R1 s \<and> commonExtraInv s"
+
+theorem "VC1 inv1 s0"
+  apply(unfold VC1_def inv1_def R1_def)
+  using cei1 VC1_def apply auto
+  done
+
+theorem cei2: "VC2 inv1 env s0 carInFront'value peCarUnder'value opened'value closed'value"
+  apply(unfold VC2_def inv1_def R1_def)
+  apply(rule impI)
+  apply(rule conjI)
+  subgoal
+   apply(unfold commonExtraInv_def)[1]
+    apply(erule conjE)+
+    using substate_toEnvNum_id[of _ s0] by force
+  using cei2 VC2_def by auto
+
+theorem cei3: "VC3 inv1 env s0 carInFront'value peCarUnder'value opened'value closed'value"
+  apply(unfold VC3_def inv1_def R1_def)
+  apply(rule impI)
+  apply(rule conjI)
+  subgoal
+   apply(unfold commonExtraInv_def)[1]
+    apply(erule conjE)+
+    using substate_toEnvNum_id[of _ s0] by force
+  using cei3 VC3_def by auto
+
+theorem cei14: "VC14 inv1 env s0 carInFront'value peCarUnder'value opened'value closed'value"
+  apply(unfold VC14_def inv1_def R1_def)
+  apply(rule impI)
+  apply(rule conjI)
+  subgoal
+   apply(unfold commonExtraInv_def)[1]
+    apply(erule conjE)+
+    using substate_toEnvNum_id[of _ s0] by force
+  using cei14 VC14_def by auto
+
+theorem cei15: "VC15 inv1 env s0 carInFront'value peCarUnder'value opened'value closed'value"
+  apply(unfold VC15_def inv1_def R1_def)
+  apply(rule impI)
+  apply(rule conjI)
+  subgoal
+   apply(unfold commonExtraInv_def)[1]
+    apply(erule conjE)+
+    using substate_toEnvNum_id[of _ s0] by force
+  using cei15 VC15_def by auto
+
+theorem cei16: "VC16 inv1 env s0 carInFront'value peCarUnder'value opened'value closed'value"
+  apply(unfold VC16_def inv1_def R1_def)
+  apply(rule impI)
+  apply(rule conjI)
+  subgoal
+   apply(unfold commonExtraInv_def)[1]
+    apply(erule conjE)+
+    using substate_toEnvNum_id[of _ s0] by force
+  using cei16 VC16_def by auto
+
+theorem cei17: "VC17 inv1 env s0 carInFront'value peCarUnder'value opened'value closed'value"
+  apply(unfold VC17_def inv1_def R1_def)
+  apply(rule impI)
+  apply(rule conjI)
+  subgoal
+   apply(unfold commonExtraInv_def)[1]
+    apply(erule conjE)+
+    using substate_toEnvNum_id[of _ s0] by force
+  using cei17 VC17_def by auto
+
+theorem cei18: "VC18 inv1 env s0 carInFront'value peCarUnder'value opened'value closed'value"
+  apply(unfold VC18_def inv1_def R1_def)
+  apply(rule impI)
+  apply(rule conjI)
+  subgoal
+   apply(unfold commonExtraInv_def)[1]
+    apply(erule conjE)+
+    using substate_toEnvNum_id[of _ s0] by force
+  using cei18 VC18_def by auto
+
+theorem cei19: "VC19 inv1 env s0 carInFront'value peCarUnder'value opened'value closed'value"
+  apply(unfold VC19_def inv1_def R1_def)
+  apply(rule impI)
+  apply(rule conjI)
+  subgoal
+   apply(unfold commonExtraInv_def)[1]
+    apply(erule conjE)+
+    using substate_toEnvNum_id[of _ s0] by force
+  using cei19 VC19_def by auto
+
+theorem cei20: "VC20 inv1 env s0 carInFront'value peCarUnder'value opened'value closed'value"
+  apply(unfold VC20_def inv1_def R1_def)
+  apply(rule impI)
+  apply(rule conjI)
+  subgoal
+   apply(unfold commonExtraInv_def)[1]
+    apply(erule conjE)+
+    using substate_toEnvNum_id[of _ s0] by force
+  using cei20 VC20_def by auto
+
+theorem cei21: "VC21 inv1 env s0 carInFront'value peCarUnder'value opened'value closed'value"
+  apply(unfold VC21_def inv1_def R1_def)
+  apply(rule impI)
+  apply(rule conjI)
+  subgoal
+   apply(unfold commonExtraInv_def)[1]
+    apply(erule conjE)+
+    using substate_toEnvNum_id[of _ s0] by force
+  using cei21 VC21_def by auto
+
+theorem cei22: "VC22 inv1 env s0 carInFront'value peCarUnder'value opened'value closed'value"
+  apply(unfold VC22_def inv1_def R1_def)
+  apply(rule impI)
+  apply(rule conjI)
+  subgoal
+   apply(unfold commonExtraInv_def)[1]
+    apply(erule conjE)+
+    apply auto
+    using substate_toEnvNum_id[of s0] by (force+)?
+  using cei22 VC22_def by auto
+
+theorem cei23: "VC23 inv1 env s0 carInFront'value peCarUnder'value opened'value closed'value"
+  apply(unfold VC23_def inv1_def R1_def)
+  apply(rule impI)
+  apply(rule conjI)
+  subgoal
+   apply(unfold commonExtraInv_def)[1]
+    apply(erule conjE)+
+    apply auto
+    using substate_toEnvNum_id[of s0] by (force+)?
+  using cei23 VC23_def by auto
+
+theorem cei24: "VC24 inv1 env s0 carInFront'value peCarUnder'value opened'value closed'value"
+  apply(unfold VC24_def inv1_def R1_def)
+  apply(rule impI)
+  apply(rule conjI)
+  subgoal
+   apply(unfold commonExtraInv_def)[1]
+    apply(erule conjE)+
+    apply auto
+    using substate_toEnvNum_id[of s0] by (force+)?
+  using cei24 VC24_def by auto
+
+theorem cei25: "VC25 inv1 env s0 carInFront'value peCarUnder'value opened'value closed'value"
+  apply(unfold VC25_def inv1_def R1_def)
+  apply(rule impI)
+  apply(rule conjI)
+  subgoal
+   apply(unfold commonExtraInv_def)[1]
+    apply(erule conjE)+
+    apply auto
+    using substate_toEnvNum_id[of s0] by (force+)?
+  using cei25 VC25_def by auto
+
+end
