WashingMachine/CommonExtraInv.thy
@@ -65,6 +65,42 @@ theorem cei43: "VC43 commonExtraInv env s0 startButton'value locked'value waterL
   apply(unfold VC43_def commonExtraInv_def)
   by simp
 
+theorem cei44: "VC44 commonExtraInv env s0 startButton'value locked'value waterLevel'value waterPresence'value temp'value freq'value"
+  apply(unfold VC44_def commonExtraInv_def)
+  by simp
+
+theorem cei45: "VC45 commonExtraInv env s0 startButton'value locked'value waterLevel'value waterPresence'value temp'value freq'value"
+  apply(unfold VC45_def commonExtraInv_def)
+  by simp
+
+theorem cei46: "VC46 commonExtraInv env s0 startButton'value locked'value waterLevel'value waterPresence'value temp'value freq'value"
+  apply(unfold VC46_def commonExtraInv_def)
+  by simp
+
+theorem cei47: "VC47 commonExtraInv env s0 startButton'value locked'value waterLevel'value waterPresence'value temp'value freq'value"
+  apply(unfold VC47_def commonExtraInv_def)
+  by simp
+
+theorem cei48: "VC48 commonExtraInv env s0 startButton'value locked'value waterLevel'value waterPresence'value temp'value freq'value"
+  apply(unfold VC48_def commonExtraInv_def)
+  by simp
+
+theorem cei49: "VC49 commonExtraInv env s0 startButton'value locked'value waterLevel'value waterPresence'value temp'value freq'value"
+  apply(unfold VC49_def commonExtraInv_def)
+  by simp
+
+theorem cei50: "VC50 commonExtraInv env s0 startButton'value locked'value waterLevel'value waterPresence'value temp'value freq'value"
+  apply(unfold VC50_def commonExtraInv_def)
+  by force
+
+theorem cei51: "VC51 commonExtraInv env s0 startButton'value locked'value waterLevel'value waterPresence'value temp'value freq'value"
+  apply(unfold VC51_def commonExtraInv_def)
+  by force
+
+theorem cei52: "VC52 commonExtraInv env s0 startButton'value locked'value waterLevel'value waterPresence'value temp'value freq'value"
+  apply(unfold VC52_def commonExtraInv_def)
+  by force
+
 theorem cei63: "VC63 commonExtraInv env s0 startButton'value locked'value waterLevel'value waterPresence'value temp'value freq'value"
   apply(unfold VC63_def commonExtraInv_def)
   by simp
@@ -94,6 +130,46 @@ theorem cei160: "VC160 commonExtraInv env s0 startButton'value locked'value wate
 theorem cei40: "VC40 commonExtraInv env s0 startButton'value locked'value waterLevel'value waterPresence'value temp'value freq'value"
   apply(unfold VC40_def commonExtraInv_def)
   by simp
+
+theorem cei132: "VC132 commonExtraInv env s0 startButton'value locked'value waterLevel'value waterPresence'value temp'value freq'value"
+  apply(unfold VC132_def commonExtraInv_def)
+  by simp
+
+theorem cei133: "VC133 commonExtraInv env s0 startButton'value locked'value waterLevel'value waterPresence'value temp'value freq'value"
+  apply(unfold VC133_def commonExtraInv_def)
+  by simp
+
+theorem cei134: "VC134 commonExtraInv env s0 startButton'value locked'value waterLevel'value waterPresence'value temp'value freq'value"
+  apply(unfold VC134_def commonExtraInv_def)
+  by simp
+
+theorem cei135: "VC135 commonExtraInv env s0 startButton'value locked'value waterLevel'value waterPresence'value temp'value freq'value"
+  apply(unfold VC135_def commonExtraInv_def)
+  by simp
+
+theorem cei136: "VC136 commonExtraInv env s0 startButton'value locked'value waterLevel'value waterPresence'value temp'value freq'value"
+  apply(unfold VC136_def commonExtraInv_def)
+  by simp
+
+theorem cei137: "VC137 commonExtraInv env s0 startButton'value locked'value waterLevel'value waterPresence'value temp'value freq'value"
+  apply(unfold VC137_def commonExtraInv_def)
+  by simp
+
+theorem cei138: "VC138 commonExtraInv env s0 startButton'value locked'value waterLevel'value waterPresence'value temp'value freq'value"
+  apply(unfold VC138_def commonExtraInv_def)
+  by simp
+
+theorem cei139: "VC139 commonExtraInv env s0 startButton'value locked'value waterLevel'value waterPresence'value temp'value freq'value"
+  apply(unfold VC139_def commonExtraInv_def)
+  by simp
+
+theorem cei140: "VC140 commonExtraInv env s0 startButton'value locked'value waterLevel'value waterPresence'value temp'value freq'value"
+  apply(unfold VC140_def commonExtraInv_def)
+  by force
+
+theorem cei141: "VC141 commonExtraInv env s0 startButton'value locked'value waterLevel'value waterPresence'value temp'value freq'value"
+  apply(unfold VC141_def commonExtraInv_def)
+  by force
 
 end
   
